Moving back to a version of config that includes qrefs

src/Base.v
@@ -778,7 +778,7 @@ Module Config.
   
   Record t := {
     dim : nat;
-    (*qrefs : Var.Map.t nat;*)
+    qrefs : Var.Map.t nat;
     qstate : Matrix dim dim
   }.
 
@@ -794,11 +794,11 @@ Module Config.
   End Refs.
   *)
 
-  Record WellScoped (refs : Var.Map.t nat) (cfg : t) := {
+  Record WellScoped (cfg : t) := {
     wf_qstate : Matrix.WF_Matrix (qstate cfg);
     wf_qrefs : List.Forall
               (fun x => snd x < dim cfg)%nat
-              (Var.Map.elements refs)
+              (Var.Map.elements (qrefs cfg))
   }.
 
   
@@ -812,32 +812,36 @@ Module Config.
 
   (* Project onto the state where qubit q is in the classical state |b> *)
   (*Definition proj q dim (b : bool) := pad_u dim q (bool_to_matrix b).*)
-  Definition measure (b : bool) (x : Var.t) refs (cfg : t)
-    : Var.Map.t nat * t :=
-    let q := find x refs in
+  Definition measure (b : bool) (x : Var.t) (cfg : t)
+    : t :=
+    let q := find x (qrefs cfg) in
     let rho' := super (pad_u q (dim cfg) (bool_to_matrix b)) (qstate cfg) in
-    (Var.Map.remove x refs, {|
+    {|
       dim := dim cfg;
+      qrefs := Var.Map.remove x (qrefs cfg);
       qstate := rho'
-    |}).
+    |}.
 
-  Definition new (b : bool) refs (cfg : t) : Var.t * Var.Map.t nat * t :=
-    let x := Var.fresh refs in
+  Definition new (b : bool) (cfg : t) : Var.t * t :=
+    let x := Var.fresh (qrefs cfg) in
     let q := dim cfg in
     let rho' := kron (qstate cfg) (bool_to_ket b) in
-    (x, Var.Map.add x q refs, {|
+    (x, {|
       dim := 1 + dim cfg;
+      qrefs := Var.Map.add x q (qrefs cfg);
       qstate := rho'
     |}).
 
   Definition apply_matrix (cfg : t) (U : Matrix (2 ^ dim cfg) (2 ^ dim cfg)) : t :=
   {|
     dim := dim cfg;
+    qrefs := qrefs cfg;
     qstate := super U (qstate cfg)
   |}.
   
 
-  Definition epr refs (cfg : t) : Var.t * Var.t * Var.Map.t nat * t :=
+  Definition epr (cfg : t) : Var.t * Var.t * t :=
+    let refs := qrefs cfg in
     let d := dim cfg in
     let x1 := Var.fresh refs in
     let refs' := Var.Map.add x1 d refs in
@@ -846,8 +850,9 @@ Module Config.
 
     let bell00 := Quantum.EPRpair † × Quantum.EPRpair in
     let rho' := kron (qstate cfg) bell00 in
-    (x1, x2, refs'', {|
+    (x1, x2, {|
       dim := 2 + dim cfg;
+      qrefs := refs'';
       qstate := rho'
     |}).
 
@@ -866,8 +871,8 @@ Module Config.
   | _, _ => Zero
   end.
 
-  Definition apply_gate (U : unitary) (xs : list Var.t) refs (cfg : t) : t :=
-    let qs := List.map (fun x => find x refs) xs in
+  Definition apply_gate (U : unitary) (xs : list Var.t) (cfg : t) : t :=
+    let qs := List.map (fun x => find x (qrefs cfg)) xs in
     apply_matrix cfg (gate_to_matrix _ U qs).
 
     
